Add operations; complete coding for cat file sys
Operations are open-a-file (getting a fd), read-a-char-from-a-fd, and
close-a-fd. There are various error conditions (some of which might map
onto exceptions). For example, opening a non-existent file might
reasonably throw something. On the other hand, attempting fgetc when at
eof plausibly should return NONE instead of SOME char at the client
level (as well as in the underlying model).

These operations now need to be lifted into values of type ffi_next,
which will operate over encoded file-system values.

compiler/bootstrap/io/catfileSystemScript.sml
@@ -1,7 +1,13 @@
 open preamble
 
+open monadsyntax
 
 val _ = new_theory "catfileSystem";
+
+val _ = overload_on ("return", ``SOME``)
+val _ = overload_on ("fail", ``NONE``)
+val _ = overload_on ("monad_bind", ``OPTION_BIND``)
+val _ = overload_on ("monad_unit_bind", ``OPTION_IGNORE_BIND``)
 
 val _ = Datatype`
   RO_fs = <| files : (string # string) list ;
@@ -9,39 +15,152 @@ val _ = Datatype`
   |>
 `
 
-val encode_files_def = Define`
-  (encode_files [] = Num 0) ∧
-  (encode_files ((s1,s2) :: t) =
-     Cons (Cons (Str s1) (Str s2)) (encode_files t))
+val nextFD_def = Define`
+  nextFD fsys = LEAST n. ~ MEM n (MAP FST fsys.infds)
 `;
-val _ = export_rewrites ["encode_files_def"]
+
+val openFile_def = Define`
+  openFile fnm fsys =
+     do
+        ALOOKUP fsys.files fnm ;
+        return <|
+          files := fsys.files ;
+          infds := (nextFD fsys, (fnm, 0)) :: fsys.infds
+        |>
+     od
+`;
+
+val A_DELKEY_def = Define`
+  A_DELKEY k alist = FILTER (λp. FST p <> k) alist
+`;
+
+val fgetc_def = Define`
+  fgetc fd fsys =
+    do
+       (fnm, off) <- ALOOKUP fsys.infds fd ;
+       content <- ALOOKUP fsys.files fnm ;
+       if off < LENGTH content then
+         return
+           (SOME (EL off content),
+            fsys with infds := (fd,(fnm,off+1)) :: A_DELKEY fd fsys.infds)
+       else
+         return (NONE, fsys)
+    od
+`;
+
+val closeFD_def = Define`
+  closeFD fd fsys =
+    do
+       ALOOKUP fsys.infds fd ;
+       return ((), fsys with infds := A_DELKEY fd fsys.infds)
+    od
+`;
+
+(* ----------------------------------------------------------------------
+    Coding RO_fs values as ffi values
+   ---------------------------------------------------------------------- *)
+
+val destStr_def = Define`
+  (destStr (Str s) = SOME s) ∧
+  (destStr _ = NONE)
+`
+val _ = export_rewrites ["destStr_def"]
+
+val destNum_def = Define`
+  (destNum (Num n) = SOME n) ∧
+  (destNum _ = NONE)
+`;
+val _ = export_rewrites ["destNum_def"]
+
+val encode_pair_def = Define`
+  encode_pair e1 e2 (x,y) = Cons (e1 x) (e2 y)
+`;
+
+val decode_pair_def = Define`
+  (decode_pair d1 d2 (Cons f1 f2) =
+      do
+        x <- d1 f1;
+        y <- d2 f2;
+        return (x,y)
+      od) ∧
+  (decode_pair _ _ _ = fail)
+`;
+
+val decode_encode_pair = Q.store_thm(
+  "decode_encode_pair",
+  `(∀x. d1 (e1 x) = return x) ∧ (∀y. d2 (e2 y) = return y) ⇒
+   ∀p. decode_pair d1 d2 (encode_pair e1 e2 p) = return p`,
+  strip_tac >> Cases >> simp[encode_pair_def, decode_pair_def])
+
+val encode_list_def = Define`
+  encode_list e l = List (MAP e l)
+`;
+
+val OPT_MMAP_def = Define`
+  (OPT_MMAP f [] = return []) ∧
+  (OPT_MMAP f (h0::t0) = do h <- f h0 ; t <- OPT_MMAP f t0 ; return (h::t) od)
+`;
+
+val decode_list_def = Define`
+  (decode_list d (List fs) = OPT_MMAP d fs) ∧
+  (decode_list d _ = fail)
+`;
+
+val decode_encode_list = Q.store_thm(
+  "decode_encode_list[simp]",
+  `(∀x. d (e x) = return x) ⇒
+   ∀l. decode_list d (encode_list e l) = return l`,
+  strip_tac >> simp[decode_list_def, encode_list_def] >> Induct >>
+  simp[OPT_MMAP_def]);
+
+val encode_files_def = Define`
+  encode_files fs = encode_list (encode_pair Str Str) fs
+`;
 
 val encode_fds_def = Define`
-  (encode_fds [] = Num 0) ∧
-  (encode_fds ((n, (fname, offset)) :: t) =
-    Cons (Cons (Num n) (Cons (Str fname) (Num offset))) (encode_fds t))
+  encode_fds fds =
+     encode_list (encode_pair Num (encode_pair Str Num)) fds
 `;
 
 val encode_def = Define`
   encode fs = cfHeapsBase$Cons (encode_files fs.files) (encode_fds fs.infds)
 `
 
-val decode_files_def = Define‘
-  (decode_files (Cons (Cons (Str s1) (Str s2)) t) = (s1,s2) :: decode_files t) ∧
-  (decode_files _ = [])
-’
-val _ = export_rewrites ["decode_files_def"]
+
+val decode_files_def = Define`
+  decode_files f = decode_list (decode_pair destStr destStr) f
+`
 
 val decode_encode_files = store_thm(
   "decode_encode_files",
-  “∀l. decode_files (encode_files l) = l”,
-  Induct >> simp[FORALL_PROD]);
-(*
-val decode_def = Define`
-  decode (Cons files fds) = <|
-    files := decode_files files ; infds := decode_fds fds
-  |>
+  “∀l. decode_files (encode_files l) = return l”,
+  simp[encode_files_def, decode_files_def] >>
+  simp[decode_encode_list, decode_encode_pair]);
+
+val decode_fds_def = Define`
+  decode_fds = decode_list (decode_pair destNum (decode_pair destStr destNum))
 `;
-*)
+
+val decode_encode_fds = Q.store_thm(
+  "decode_encode_fds",
+  `decode_fds (encode_fds fds) = return fds`,
+  simp[decode_fds_def, encode_fds_def] >>
+  simp[decode_encode_list, decode_encode_pair]);
+
+val decode_def = Define`
+  (decode (Cons files0 fds0) =
+     do
+        files <- decode_files files0 ;
+        fds <- decode_fds fds0 ;
+        return <| files := files ; infds := fds |>
+     od) ∧
+  (decode _ = fail)
+`;
+
+val decode_encode_FS = Q.store_thm(
+  "decode_encode_FS",
+  `decode (encode fs) = return fs`,
+  simp[decode_def, encode_def, decode_encode_files, decode_encode_fds] >>
+  simp[theorem "RO_fs_component_equality"]);
 
 val _ = export_theory();
